VSU with smax_prog now working; top-level file: verif_linked_main / verif_linked_fastmain

progs/VSUpile/verif_core.v
@@ -3,14 +3,20 @@ Require Import VST.floyd.VSU.
 
 Require Import VST.floyd.linking.
 
-Require Import verif_stdlib. (*M is a parameter of that module, so we're getting access to it now*)
-Require Import spec_pile_private.
+Require Import spec_stdlib.
 
+Require Import verif_stdlib.
 Require Import verif_pile.
-Definition PILE := (*verif_pile.*)PILEPRIV M.
-
 Require Import verif_onepile.
-Definition ONEPILE := verif_onepile.ONEPILE PILE.
+Require Import verif_apile.
+Require Import verif_triang.
+
+Section CORE_VSU.
+Variable M: MallocFreeAPD.
+Definition PrivPILE: spec_pile_private.PilePrivateAPD M:= PILEPRIV M.
+Definition PILE: spec_pile.PileAPD := spec_pile_private.pilepreds PrivPILE. 
+
+Definition ONEPILE : spec_onepile.OnePileAPD := ONEPILE PILE.
 
 Definition onepile_pile_prog: Clight.program := 
   match link_progs pile.prog onepile.prog with
@@ -26,8 +32,7 @@ Instance mrg_cs1 : compspecs. make_compspecs mrg_prog1. Defined.
 
 Definition mrg_Vprog1:varspecs. mk_varspecs mrg_prog1. Defined.
 
-(*unresolved imports*)
-Definition mrg_Imports1:funspecs := MF_ASI.
+Definition mrg_Imports1:funspecs := (MF_ASI M).
 
 Definition mrg_Exports1:funspecs := 
 G_merge (spec_pile.PileASI M PILE) (spec_onepile.OnepileASI M ONEPILE).
@@ -39,8 +44,7 @@ Proof.
   VSUMerge (PilePrivateVSU M) (OnepileVSU M PILE).
 Qed.
 
-Require Import verif_apile.
-Definition APILE := verif_apile.APILE M PILE.
+Definition APILE := verif_apile.APILE M PrivPILE.
 
 Definition apile_onepile_pile_prog: Clight.program := 
   match link_progs mrg_prog1 apile.prog with
@@ -57,20 +61,17 @@ Instance mrg_cs2 : compspecs. make_compspecs mrg_prog2. Defined.
 
 Definition mrg_Vprog2:varspecs. mk_varspecs mrg_prog2. Defined.
 
-(*unresolved imports*)
-Definition mrg_Imports2:funspecs := MF_ASI.
+Definition mrg_Imports2:funspecs := MF_ASI M.
 
-Definition mrg_Exports2:funspecs := G_merge  mrg_Exports1 (Apile_ASI M PILE).
+Definition mrg_Exports2:funspecs := G_merge  mrg_Exports1 (Apile_ASI M PrivPILE).
 
 Definition Apile_Onepile_Pile_VSU:
 @VSU NullExtension.Espec
    mrg_Vprog2 mrg_cs2 nil mrg_Imports2 mrg_prog2 mrg_Exports2.
 Proof.
-  VSUMerge (Onepile_Pile_VSU) (ApileVSU M PILE).
+  VSUMerge (Onepile_Pile_VSU) (ApileVSU M PrivPILE).
   intuition.
 Qed.
-
-Require Import verif_triang.
 
 Definition triang_apile_onepile_pile_prog: Clight.program := 
   match link_progs mrg_prog2 triang.prog with
@@ -87,8 +88,7 @@ Instance mrg_cs3 : compspecs. make_compspecs mrg_prog3. Defined.
 
 Definition mrg_Vprog3:varspecs. mk_varspecs mrg_prog3. Defined.
 
-(*unresolved imports*)
-Definition mrg_Imports3:funspecs := MF_ASI.
+Definition mrg_Imports3:funspecs := MF_ASI M.
 
 Definition mrg_Exports3:funspecs := G_merge mrg_Exports2 (spec_triang.TriangASI M).
 
@@ -116,16 +116,19 @@ Definition coreVprog:varspecs. mk_varspecs coreprog. Defined.
 
 Definition coreImports:funspecs := nil.
 
-Definition coreExports:funspecs := G_merge MF_ASI mrg_Exports3.
+Definition coreExports:funspecs := G_merge (MF_ASI M) mrg_Exports3.
 
-Definition MM_Triang_Apile_Onepile_Pile_VSU:
-@VSU NullExtension.Espec coreVprog coreCS MF_E coreImports coreprog coreExports.
+Definition coreBuiltins:funspecs := (MallocFreeASI M). (*i.e. MF_E M*)
+
+Definition Core_VSU:
+@VSU NullExtension.Espec coreVprog coreCS coreBuiltins coreImports coreprog coreExports.
 Proof.
-  VSUMerge MallocFreeVSU (Triang_Apile_Onepile_Pile_VSU). congruence.
+  VSUMerge (MallocFreeVSU M) (Triang_Apile_Onepile_Pile_VSU). congruence.
 Qed.
 
-Definition CoreVSU: @CanonicalVSU NullExtension.Espec
-   coreVprog coreCS MF_E coreImports coreprog coreExports.
+Definition Core_CanVSU: @CanonicalVSU NullExtension.Espec
+   coreVprog coreCS coreBuiltins coreImports coreprog coreExports.
 Proof.
-eapply VSU_to_CanonicalVSU. apply MM_Triang_Apile_Onepile_Pile_VSU.
+eapply VSU_to_CanonicalVSU. apply Core_VSU.
 Qed.
+End CORE_VSU.
